common/Exec.v
@@ -426,9 +426,9 @@ Definition do_ef_debug (cp: compartment) (kind: positive) (text: ident) (targs: 
        (w: world) (vargs: list val) (m: mem) : option (world * trace * val * mem) :=
   Some(w, E0, Vundef, m).
 
-Definition do_builtin_or_external (name: string) (sg: signature)
+Definition do_builtin_or_external (name: string) (cp: compartment) (sg: signature)
        (w: world) (vargs: list val) (m: mem) : option (world * trace * val * mem) :=
-  match lookup_builtin_function name sg with
+  match lookup_builtin_function name cp sg with
   | Some bf => match builtin_function_sem bf vargs with Some v => Some(w, E0, v, m) | None => None end
   | None    => do_external_function name sg ge w vargs m
   end.
@@ -437,8 +437,8 @@ Definition do_external (ef: external_function):
        world -> list val -> mem -> option (world * trace * val * mem) :=
   match ef with
   | EF_external cp name sg => do_external_function name sg ge
-  | EF_builtin cp name sg => do_builtin_or_external name sg
-  | EF_runtime cp name sg => do_builtin_or_external name sg
+  | EF_builtin cp name sg => do_builtin_or_external name cp sg
+  | EF_runtime cp name sg => do_builtin_or_external name cp sg
   | EF_vload cp chunk => do_ef_volatile_load cp chunk
   | EF_vstore cp chunk => do_ef_volatile_store cp chunk
   | EF_malloc cp => do_ef_malloc cp
@@ -459,11 +459,11 @@ Proof with try congruence.
   assert (SIZE: forall v sz, do_alloc_size v = Some sz -> v = Vptrofs sz).
   { intros until sz; unfold Vptrofs; destruct v; simpl; destruct Archi.ptr64 eqn:SF;
     intros EQ; inv EQ; f_equal; symmetry; eauto with ptrofs. }
-  assert (BF_EX: forall name sg,
-    do_builtin_or_external name sg w vargs m = Some (w', t, vres, m') ->
-    builtin_or_external_sem name sg ge vargs m t vres m' /\ possible_trace w t w').
+  assert (BF_EX: forall name cp sg,
+    do_builtin_or_external name cp sg w vargs m = Some (w', t, vres, m') ->
+    builtin_or_external_sem name cp sg ge vargs m t vres m' /\ possible_trace w t w').
   { unfold do_builtin_or_external, builtin_or_external_sem; intros.
-    destruct (lookup_builtin_function name sg ) as [bf|].
+    destruct (lookup_builtin_function name cp sg ) as [bf|].
   - destruct (builtin_function_sem bf vargs) as [vres1|] eqn:BF; inv H.
     split. constructor; auto. constructor.
   - eapply do_external_function_sound; eauto.
@@ -527,11 +527,11 @@ Proof.
   { unfold Vptrofs, do_alloc_size; intros; destruct Archi.ptr64 eqn:SF.
     rewrite Ptrofs.of_int64_to_int64; auto.
     rewrite Ptrofs.of_int_to_int; auto. }
-  assert (BF_EX: forall name sg,
-    builtin_or_external_sem name sg ge vargs m t vres m' ->
-    do_builtin_or_external name sg w vargs m = Some (w', t, vres, m')).
+  assert (BF_EX: forall name cp sg,
+    builtin_or_external_sem name cp sg ge vargs m t vres m' ->
+    do_builtin_or_external name cp sg w vargs m = Some (w', t, vres, m')).
   { unfold do_builtin_or_external, builtin_or_external_sem; intros.
-    destruct (lookup_builtin_function name sg) as [bf|].
+    destruct (lookup_builtin_function name cp sg) as [bf|].
   - inv H1. inv H0. rewrite H2. auto.
   - eapply do_external_function_complete; eauto.
   }
